{x}+{x}xx = {x}+{x} = x = x = {{{x}^{2}}+{x}}+{2} = {{x}^{2}}+{x} = {x}^{2} = x = x = 2 = \frac{x}{x} = x = x = \frac{{{x}^{3}}+{3}}{x} = {{x}^{3}}+{3} = {x}^{3} = x = 3 = x = {x}^{x} = x = x = {x}^{{x}^{x}} = x = {x}^{x} = x = x = {{sin({x})}+{tg({x})}}+{{3}*{x}} = {sin({x})}+{tg({x})} = sin({x}) = x = tg({x}) = x = {3}*{x} = 3 = x = ({{sin({x})}+{tg({x})}}+{{3}*{x}})^{\frac{1}{x}} = {{sin({x})}+{tg({x})}}+{{3}*{x}} = {sin({x})}+{tg({x})} = sin({x}) = x = tg({x}) = x = {3}*{x} = 3 = x = \frac{1}{x} = 1 = x = ({{sin({x})}+{tg({x})}}+{{3}*{x}})^{\frac{1}{x}} = {{sin({x})}+{tg({x})}}+{{3}*{x}} = {sin({x})}+{tg({x})} = sin({x}) = x = tg({x}) = x = {3}*{x} = 3 = x = \frac{1}{x} = 1 = x = ({{sin({x})}+{tg({x})}}+{{3}*{x}})^{\frac{1}{x}} = {{sin({x})}+{tg({x})}}+{{3}*{x}} = {sin({x})}+{tg({x})} = sin({x}) = x = tg({x}) = x = {3}*{x} = 3 = x = \frac{1}{x} = 1 = x